dump

PartialMonad.lean
@@ -1,33 +1,38 @@
 import «PartialMonad».Basic
 
 inductive PartialStep (σ : Type u) (α : Type v) : Type (max u v)
-  | step (nextState : σ)
+  | running (nextState : σ)
   | complete (result : α)
 
 namespace PartialStep
 
 def map (f_state : σ → σ') (f_result : α → α') : PartialStep σ α → PartialStep σ' α'
-  | .step s => .step <| f_state s
+  | .running s => .running <| f_state s
   | .complete r => .complete <| f_result r
 
 end PartialStep
 
-structure PartialM.Raw.StateMachine (α : Type u) : Type (u+1) where
-  {σ : Type u}
+structure PartialM.Raw.StateMachine.{u, v} (α : Type u) : Type (max u (v+1)) where
+  {σ : Type v}
   (next : σ → PartialStep σ α)
 
 structure PartialM.Raw (α : Type u) extends Raw.StateMachine α where
   (state : σ)
 
-/-- `RawFun α β` represents a function `α → Raw β` in such a way that we can quotient it, by
-summing all possible states into one state machine, and letting the initial state depend on some
-value `a : α` -/
-structure PartialM.RawFun (α : Type u) (β : Type v) extends Raw.StateMachine (ULift β) where
-  (stateFun : α → σ)
+/-
+I was hoping to simplify things by mandating that the state type `σ` always lives in `Type`,
+however, that precludes us from using a dependent sum `Σ (a : α), _` as a state in `bind`, since `α`
+lives in an arbitrary universe `Type u`, the dependent sum will live at least in `u` as well.
 
-def PartialM.RawFun.apply (f : RawFun α β) (a : α) : (PartialM.Raw β) where
-  toStateMachine := f.toStateMachine
-  state := f.stateFun a
+I really don't want a hidden universe parameter for the state type,
+so instead I've tied the state type to live in the same universe as the parameter `α`, and
+changed `bind` to have `α` and `β` live in the same universe.
+In fact, `Bind.bind` also has `α` and `β` in the same universe, so the previous heterogenous version
+was more general than required anyway.
+
+So far, this works
+-/
+
 
 namespace PartialM.Raw
 
@@ -41,36 +46,158 @@ def pure (x : α) : PartialM.Raw α where
   state := ()
   next _ := .complete x
 
-/-- `ofFun f` turns a `f : α → Raw β` into the equivalent `RawFun α β`  -/
-def ofFun {α : Type u} {β : Type v} (f : α → Raw β) : RawFun α β where
-  σ := Σ a, (f a).σ
-  next := fun ⟨a, s⟩ => (f a).next s |>.map (⟨_, ·⟩) id
-  stateFun := fun a => ⟨_, (f a).state⟩
+#check ULift
 
-def bindAux (x : PartialM.Raw α) (f : PartialM.RawFun α β) : PartialM.Raw β where
-  σ := x.σ ⊕ f.σ
-  -- /-^^^---^^^
+/-- `map f x` applies a pure function `f : α → β` to the final result of state machine `x`,
+after it has completed.
+It is allowed for `β` to live in a higher universe from `α`, but not a lower one -/
+-- def map {α : Type u} {β : Type (max u v)} (f : α → β) (x : PartialM.Raw α) : PartialM.Raw β where
+--   state := ULift.up.{v} x.state
+--   next s := match x.next s.down with
+--     | .running s => .running (.up s)
+--     | .complete a => .complete (f a)
+def map {α : Type u} {β : Type v} (f : α → β) (x : PartialM.Raw α) : PartialM.Raw β where
+  state := x.state
+  next s := match x.next s with
+    | .running s => .running (s)
+    | .complete a => .complete (f a)
+
+def nextState (x : PartialM.Raw α) : PartialStep (PartialM.Raw α) α :=
+  (x.next x.state).map (fun state => {x with state}) id
+
+open PartialStep in
+def iterate (x : PartialM.Raw α) : Nat → PartialStep (PartialM.Raw α) α
+  | 0    => running x
+  | n+1  => match x.nextState with
+    | running x => x.iterate n
+    | complete a => complete a
+
+theorem iterate_succ (x : PartialM.Raw α) (n : Nat) :
+    x.iterate (n+1) = match (x.iterate n) with
+      | .running x => x.nextState
+      | .complete a => .complete a := by
+  induction n generalizing x
+  case zero =>
+    simp only [iterate]
+    split <;> simp_all
+  case succ n ih =>
+    stop
+    rw [iterate]
+    -- rcases h_iterate_n : x.iterate n with x_n | a
+    rcases h_nextState : x.nextState with x'|a
+    · simp
+    · simp
+    -- · simp [h_iterate_n] at ih
+    --   rcases h_nextState : x.nextState with x' | a'
+    --   · simp [iterate, h_nextState]
+    --   · simp_all
+    -- · sorry
+
+/-- `x.CompletesInNSteps n` holds if the state machine `x` yields a value in at most `n` steps -/
+def CompletesInNSteps (x : Raw α) (n : Nat) : Prop := ∃ a, x.iterate n = .complete a
+
+/-- If a state machine is known to complete in a finite number of steps, we can compute it's result
+ -/
+def getOfCompletes (x : Raw α) {n} (h : x.CompletesInNSteps n) : α :=
+  match hi : x.iterate n with
+    | .running _ => False.elim <| by simp_all [CompletesInNSteps]
+    | .complete a => a
+
+/-
+> [!todo]
+> We could generalize `CompletesInNSteps` to just `CompletesInFiniteTime`, by moving the `n` into
+> an existential in the property, as in ``
+> ```lean
+> def CompletesInFiniteTime (x : Raw α) : Prop := ∃ n a, x.iterate n = .complete a
+> ```
+> We can then write `getOfCompletes` as a function which matches on `x.nextStep`, and recursively
+> calls itself in the `running` branch, using the proof of completion to show that this terminates.
+>
+> This then leads to a nice noncomputable `toOption` implementation, by using `Classical.em` on
+> `x.CompletesInFiniteTime`
+-/
+
+/-- `join x` collapses a nested state-machine `x : Raw (Raw σ)` into a single state machine `Raw α`.
+Operationally, `join x` first runs `x` until it yields the inner state machine,
+which is then run until completion as well -/
+def join {α : Type u} (x : PartialM.Raw.{u+1,u} (PartialM.Raw.{u,u} α)) : PartialM.Raw.{u,u} α where
+  σ := {state : x.σ × Nat // x.iterate state.2 = .running {x with state := state.1}}
+       ⊕ Σ' (n : Nat) (h : x.CompletesInNSteps n), (x.getOfCompletes h).σ
+  -- /-  ^^^^^^^^^^^^^^^^^^^^^^^^^^^^^^^^^^^^^^^^^^^^^^^^^^^^^^^^^^^^^^^^
+  -- | The state of `join x` is the sum of states of the outer state machine `x`, and
+  -- | the states of the nested state machine that is yielded by `x`
+  -- | However, we don't actually know the type of states that this inner machine has, a-priori.
+  -- | So, read "the states of the nested state machine" as: the states of the state machine
+  -- | returned by `x` in `n` steps, assuming that `x` indeed terminates in `n` steps.
+  -- | Then, to actually be able to transition into one of these nested states, we have to show
+  -- | that `x` indeed terminates, so we track for the states of `x`, those on the LHS of the sum,
+  -- | that indeed we only enter states which are reachable from `x`'s starting state
+  state := .inl ⟨⟨x.state, 0⟩, rfl⟩
+  next  := fun
+    | .inl ⟨⟨(s : x.σ), n⟩, hs⟩ =>
+      .running <| match hs' : x.next s with
+        | .running s'    => .inl ⟨(s', n+1), by simp [iterate_succ, nextState, hs, hs']; rfl⟩
+        -- ^^^^^^^^ If `x` is still `running`, continue with the next state of `x`
+        | .complete inner =>
+        -- ^^^^^^^^ Otherwise, if `x` has completed,
+        --          go to the first state of the nested state machine
+          have h_complete := by
+            simp only [CompletesInNSteps, iterate_succ, hs, nextState, hs']
+            exact ⟨inner, rfl⟩
+          have h_cast := by
+            simp [getOfCompletes]
+            split
+            next => exfalso; apply getOfCompletes.proof_1; repeat assumption
+            next h =>
+              simp only [iterate_succ, hs, nextState, hs'] at h
+              change PartialStep.complete inner = _ at h
+              injection h with h
+              rw [h]
+          .inr <| ⟨n+1, h_complete, cast h_cast inner.state⟩
+    | .inr ⟨n, h, s⟩ => ((x.getOfCompletes h).next s).map (.inr ⟨n, h, ·⟩) id
+    -- ^^^^^^^^^^^^^^^^^^^^^^ Finally, run `f` until completion, mapping its state into
+    --                        the combined sum state each step
+
+-- > [!todo]
+-- > The setup of `join` is pretty bad. Fixing the state `σ` to live in `Type`, while the return
+-- > type may live in arbitrary universes, means that we are not able to store the state-transition
+-- > function of the nested state machine in the state of the combined state machine.
+-- > Instead, we can only store the proof that the outer machine terminates in `n` steps, and then
+-- > re-run the outer state machine until completion for each step of the nested state machine.
+-- >
+-- > There is some hope that in an eventual "`PartialM.run`" function, the loop that repeatedely
+-- > polls the `join` state machine gets inline, so that `CSE` can kick in, and the outer state machine
+-- > might not actually be re-run for every step, but having to rely on this series of "hopes" and
+-- > "mights" makes me nervous
+-- >
+-- > I attempted to fix things by introducing a new universe level for the state, in the hopes of
+-- > keeping this an internal implementation detail, but, actually storing a state machine in the
+-- > `join` result would require a universe bump of the state universe.
+-- > This is an unacceptable leak of universe levels, I'm sticking with the computationally horrible
+-- > recomputation for now
+
+/-- `bind x f`, composes two state machines together, by running `f` after `x` completes,
+where the second state machine, `f`, may depend on the result of `x`  -/
+def bind {α β : Type u} (x : PartialM.Raw α) (f : α → PartialM.Raw β) : PartialM.Raw β where
+  σ := x.σ ⊕ Σ (a : α), (f a).σ
+  -- /-^^^---^^^^^^^^^^^^
   -- | The state of `bind x f` is the sum of states of `x` and `f`
   -- | However, `f` is a *function*, not a straight state machine,
   -- | so read "the states of `f`" as:
   -- |   "the infinite sum of all state types `(f x').σ`, for all possible values `a : α`"
+  -- |
   state := .inl x.state
   next := fun
-    | .inl s      =>
-      .step <| match x.next s with
-        | .step s'    => .inl s'
-        -- ^^^^^^^ If `x` is still going, `step` into the next state of `x`
-        | .complete a => .inr <| f.stateFun a
+    | .inl (s : x.σ) =>
+      .running <| match x.next s with
+        | .running s'    => .inl s'
+        -- ^^^^^^^ If `x` is still going, `running` into the next state of `x`
+        | .complete a => .inr <| ⟨_, (f a).state⟩
         -- ^^^^^^^ Otherwise, if `x` has completed, and yielded some value `a`,
-        --         `step` into the first state of `f` that corresponds to `a`
-    | .inr s => (f.next s).map .inr id
+        --         step into the first state of `f` that corresponds to `a`
+    | .inr ⟨a, s⟩ => ((f a).next s).map (.inr ⟨_, ·⟩) id
     --          ^^^^^^^^^^^^^^^^^^^^^^ Finally, run `f` until completion, mapping its state into
     --                                 the combined sum state each step
-
-/-- `bind x f`, composes two state machines together, by running `f` after `x` completes,
-where the second state machine, `f`, may depend on the result of `x`  -/
-def bind (x : PartialM.Raw α) (f : α → PartialM.Raw β) : PartialM.Raw β :=
-  bindAux x (ofFun f)
 
 instance : Monad (PartialM.Raw) where
   pure := pure
@@ -111,7 +238,7 @@ state machines internal detail.
 Thus, we quotient through a bisimilarity relation, to hide these internal states. -/
 
 inductive PartialStepAgrees (R : σ₁ → σ₂ → Prop) : PartialStep σ₁ α → PartialStep σ₂ α → Prop
-  | step {s₁ s₂} : R s₁ s₂ → PartialStepAgrees R (.step s₁) (.step s₂)
+  | running {s₁ s₂} : R s₁ s₂ → PartialStepAgrees R (.running s₁) (.running s₂)
   | complete {a} : PartialStepAgrees R (.complete a) (.complete a)
 
 def IsBisimulation {x y : Raw.StateMachine α} (R : x.σ → y.σ → Prop) : Prop :=
@@ -186,107 +313,8 @@ end BisimIsEquiv
 
 end Raw
 
-/-! The notion of `Bisim`ilarity generalizes to `RawFun` -/
-inductive RawFun.Bisim (x y : PartialM.RawFun α β) : Prop where
-  | mk
-    (R : x.σ → y.σ → Prop)
-    (bisim : Raw.IsBisimulation R)
-    (state : ∀ a, R (x.stateFun a) (y.stateFun a))
-
-/-! `RawFun.Bisim`, too, is an equivalence -/
-namespace RawFun.Bisim
-open PartialM (RawFun)
-open PartialM.Raw (isBisimulation_eq)
-
-
-theorem rfl (x : RawFun α β) : Bisim x x :=
-  .mk Eq isBisimulation_eq (by intro; rfl)
-
-theorem trans : Bisim x y → Bisim y z → Bisim x z
-  | ⟨R₁, bisim₁, state₁⟩, ⟨R₂, bisim₂, state₂⟩ =>
-    .mk
-      (R := fun x z => ∃ y, R₁ x y ∧ R₂ y z)
-      (state := fun a => ⟨y.stateFun a, state₁ a, state₂ a⟩)
-      (bisim := by
-        intro s₁ s₃
-        simp
-        intro s₂ hR₁ hR₂
-        specialize bisim₁ _ _ hR₁; revert bisim₁
-        specialize bisim₂ _ _ hR₂; revert bisim₂
-
-        rcases x.next s₁ with s₁'|a₁
-        <;> rcases y.next s₂ with s₂'|a₂
-        <;> rcases z.next s₃ with s₃'|a₃
-        <;> rintro ⟨next₂⟩ ⟨next₁⟩
-        <;> constructor
-        exact ⟨_, next₁, next₂⟩
-      )
-
-theorem symm : Bisim x y → Bisim y x
-  | ⟨R, bisim, state⟩ =>
-      .mk (R := fun s₂ s₁ => R s₁ s₂) (state := state) (bisim := by
-        intros s₁ s₂ hR
-        specialize bisim _ _ hR
-        revert bisim
-        cases x.next s₂ <;> cases y.next s₁
-        <;> rintro ⟨bisim⟩
-        <;> constructor
-        assumption
-      )
-
-def equivalence : Equivalence (Bisim (α := α) (β := β)) where
-  refl := rfl
-  trans := trans
-  symm := symm
-
-end RawFun.Bisim
-
-instance RawFun.setoid (α β : Type) : Setoid (PartialM.RawFun α β) where
-  r := Bisim
-  iseqv := Bisim.equivalence
-
 /-- TODO: describe `PartialM` -/
-def PartialM (α : Type u) : Type (u+1) := Quotient (PartialM.Raw.setoid α)
-
-/-- `PartialFun α β` represents a function `α → PartialM β` -/
-def PartialFun (α β : Type) : Type 1 := Quotient (RawFun.setoid α β)
-
-namespace PartialFun
-
-def apply (f : PartialFun α β) : α → PartialM β := fun a =>
-  Quotient.liftOn f (fun rf => Quotient.mk _ <| rf.apply a) <| by
-    rintro rf₁ rf₂ ⟨R, bisim, stateFun⟩
-    apply Quotient.sound
-    exact ⟨R, bisim, stateFun _⟩
-
-#check Raw.bind
-
-/-!
-  How do I actually define `mk`?
-  I assume I have to go through `Quotient.lift`, or one of it's variants, somehow, but those
-  all operate on `x : Quotient _`, but what I have is a function `f : α → Quotient _`
-
-  Mathlib has [`Quotient.choice`](https://leanprover-community.github.io/mathlib4_docs/Mathlib/Data/Quot.html#Quotient.choice),
-  which does what i want, but is noncomputable, and
-  [`Quotient.finChoice`](https://leanprover-community.github.io/mathlib4_docs/Mathlib/Data/Fintype/Quotient.html#Quotient.finChoice),
-  which is computable, but only works if the argument of the function-type is a finite type.
-
-  The fact that `Quotient.choice` is exactly the signature I need, makes me suspect that it is
-  fundamentally impossible to do this computably.
-
-  That means, I could only define `bind` over `PartialM α` when `α` is a finite type.
-  Thus, `PartialM` would not be a true `Monad` (since `Monad` mandates a `Type u → Type v` signature,
-  it leaves no room for the extra `Fintype` assumption).
-
-  `Raw : Type → Type`
-
--/
-
-def mk (f : α → PartialM β) : PartialFun α β :=
-  -- Quotient.hrecOn _ _ _
-  sorry
-
-end PartialFun
+def PartialM.{u} (α : Type u) : Type _ := Quotient (PartialM.Raw.setoid.{u,0} α)
 
 namespace PartialM
 
@@ -295,12 +323,6 @@ def ofRaw : PartialM.Raw α → PartialM α := Quotient.mk _
 
 def pure (a : α) : PartialM α :=
   .ofRaw <| Raw.pure a
-
-def Raw.map (f : α → β) (x : PartialM.Raw α) : PartialM.Raw β where
-  state := x.state
-  next s := match x.next s with
-    | .step s => .step s
-    | .complete a => .complete (f a)
 
 def map (f : α → β) (x : PartialM α) : PartialM β :=
   Quotient.liftOn x (ofRaw ∘ Raw.map f) <| by
@@ -320,7 +342,10 @@ def Raw.join : PartialM.Raw (PartialM.Raw α) → PartialM.Raw α :=
   (Raw.bind · (fun (x : PartialM.Raw α) => x))
 
 def join (x : PartialM (PartialM α)) : PartialM α :=
-  Quotient.liftOn x _ _
+  let f_lift (x : Raw (PartialM α)) : PartialM α :=
+    -- let xf := x.map _
+  have h_lift_sound := by sorry
+  Quotient.liftOn x f_lift h_lift_sound
 
 def bind (x : PartialM α) (f : α → PartialM β) : PartialM β :=
   let bind_f (x : PartialM.Raw α) : PartialM β :=
