PartialDSL.lean
@@ -1,0 +1,162 @@
+import Std.Data.Sum.Basic
+
+/-!
+
+Including the type of states `σ` and the transition function into the `PartialM` monad requires a
+universe bump. This universe bump causes all kinds of problems when trying to define `PartialM.bind`.
+
+Thus, in this file we explore an alternative idea, we keep the state type external, as a parameter
+to `PartialM`.
+Then, we lose the ability to compose partial computations from different statemachines
+together with just `do`-notation, so we recover this with a specialized `partial` dsl.
+
+Sadly, I'm not sure that `PartialStateM σ : Type → Type`, for some fixed state `σ` is a monad.
+How would we define `pure`, without being able to control the state machine?
+In fact, how do we even
+
+-/
+
+structure PartialStateM.Raw (σ α : Type) :
+    Type where
+  state : σ
+  next : σ → σ ⊕ α
+
+namespace PartialStateM.Raw
+
+def nextState (x : Raw σ α) : Raw σ α ⊕ α :=
+  x.next x.state |>.map ({x with state := ·}) id
+
+def pure {σ : Type} [Inhabited σ] {α} (a : α) : Raw σ α where
+  state := default
+  next := fun _ => .inr a
+
+/-!
+Side Note: `pure` is the reason we store `next` in `Raw` as well,
+rather than having a fixed transition function determined by `σ`.
+
+If we did the latter, then both the state space and the computation would be fixed,
+we could only pick the state at which to start the computation. This means that the choice of `σ`
+would also determine the output type `α`, hence, there would be no way to define `pure` as above.
+
+We could make `next` a parameter to `Raw` as well, but then could only define `pure` for
+particular values of `next`, where in particular `next` depends on `α`,
+so we still would not get a proper `Monad` instance. -/
+
+def map (f : α → β) (x : Raw σ α) : Raw σ β where
+  state := x.state
+  next s := match x.next s with
+    | .inl s' => .inl s'
+    | .inr a  => .inr (f a)
+
+instance : Functor (Raw σ) where
+  map := map
+
+/-- `join x` collapses a nested state-machine `x : Raw (Raw σ)` into a single state machine `Raw α`.
+Operationally, `join x` first runs `x` until it yields the inner state machine,
+which is then run until completion as well -/
+def join (x : Raw σ₁ (Raw σ₂ α)) : Raw (σ₁ ⊕ Raw σ₂ α) α where
+  state := .inl x.state
+  next := fun
+    | .inl s₁ => .inl <| x.next s₁
+    | .inr s₂ => s₂.nextState |> Sum.map .inr id
+
+/-!
+## A note on homogeneous join
+Even if we know that `σ₁ = σ₂`, we are not automatically able to join this into a state machine
+with the same state space.
+This is because the nested state machine might use a different transition function, so we actually
+need to store the nested transition function as well.
+
+(I guess this would be a good argument for externalising the transition function as well, but then
+ how do we define `pure`?)
+-/
+
+def bind (x : Raw σ₁ α) (f : α → Raw σ₂ β) : Raw (σ₁ ⊕ (Raw σ₂ β)) β :=
+  (x.map f).join
+
+
+section BisimSection
+
+def IsBisimulation (x : Raw σ₁ α) (y : Raw σ₂ α) (R : σ₁ → σ₂ → Prop) : Prop :=
+  ∀ (s₁ : σ₁) (s₂ : σ₂), R s₁ s₂ → (Sum.LiftRel R Eq) (x.next s₁) (y.next s₂)
+
+inductive Bisim (x : Raw σ₁ α) (y : Raw σ₂ α) : Prop where
+  | mk
+    (R : σ₁ → σ₂ → Prop)
+    (bisim : IsBisimulation x y R)
+    (state : R x.state y.state)
+
+/-! `Bisim` is an equivalence -/
+section BisimIsEquiv
+
+theorem isBisimulation_eq {x : Raw σ α} : IsBisimulation x x Eq := by
+  simp only [IsBisimulation, forall_eq', implies_true]
+  intro s; cases x.next s <;> (constructor; rfl)
+
+namespace Bisim
+
+theorem rfl (x : Raw σ α) : Bisim x x :=
+  .mk Eq isBisimulation_eq (by rfl)
+
+theorem trans : Bisim x y → Bisim y z → Bisim x z
+  | ⟨R₁, bisim₁, state₁⟩, ⟨R₂, bisim₂, state₂⟩ =>
+    .mk
+      (R := fun x z => ∃ y, R₁ x y ∧ R₂ y z)
+      (state := ⟨y.state, state₁, state₂⟩)
+      (bisim := by
+        intro s₁ s₃
+        simp
+        intro s₂ hR₁ hR₂
+        specialize bisim₁ _ _ hR₁; revert bisim₁
+        specialize bisim₂ _ _ hR₂; revert bisim₂
+
+        rcases x.next s₁ with s₁'|a₁
+        <;> rcases y.next s₂ with s₂'|a₂
+        <;> rcases z.next s₃ with s₃'|a₃
+        <;> rintro ⟨next₂⟩ ⟨next₁⟩
+        <;> constructor
+        · exact ⟨_, next₁, next₂⟩
+        · simp_all
+      )
+
+theorem symm : Bisim x y → Bisim y x
+  | ⟨R, bisim, state⟩ =>
+      .mk (R := fun s₂ s₁ => R s₁ s₂) (state := state) (bisim := by
+        intros s₁ s₂ hR
+        specialize bisim _ _ hR
+        revert bisim
+        cases x.next s₂ <;> cases y.next s₁
+        <;> rintro ⟨bisim⟩
+        <;> constructor
+        · assumption
+        · simp_all
+      )
+
+def equivalence : Equivalence (Bisim (σ₁ := σ) (σ₂ := σ) (α := α)) where
+  refl := rfl
+  trans := trans
+  symm := symm
+
+end Bisim
+
+instance setoid (α : Type _) : Setoid (Raw σ α) where
+  r := Bisim
+  iseqv := Bisim.equivalence
+
+end BisimIsEquiv
+end BisimSection
+
+end Raw
+
+/-
+So far, so good, but we already highlighted that there is no hope for a `Monad` instance here.
+The whole reason for bothering with quotients, is that they were required to make the `Monad`
+instance on raw state machines (with bundled state types) lawful.
+If we don't have a Monad instance to begin with, what's the point?
+
+I guess there is still the benefit of it being the proper thing to do, so that equality does not
+distinguish what we don't want distuinguished.
+
+However, for LeanMLIR the quotient might not even be necessary:
+We can just define the refinement relation on partial computations to consider bisimular
+computations refinements of eachother, thus side-stepping the mis-behaving equality -/
