PartialMonad/CoroutineM.lean
@@ -1,0 +1,67 @@
+import Std.Data.Sum.Basic
+
+/-!
+This file defines the `CoroutineM` monad.
+
+A coroutine is a suspendable, potentially non-terminating computation.
+Note that this file defines such coroutines directly in terms of state machines,
+which means different computations resulting in the same final value are not necessarily equal.
+In particular, this monad is *not* an instance of `LawfulMonad`.
+
+For a lawful, but more complicated version, see `LawfulCoroutineM`
+
+-/
+
+structure CoroutineM (α : Type u) : Type (u+1) where
+  {σ : Type u}
+  (next : σ → σ ⊕ α)
+  (state : σ)
+
+namespace CoroutineM
+
+/-- Runs the coroutine for a single step -/
+def nextState (x : CoroutineM α) : (CoroutineM α) ⊕ α :=
+  (x.next x.state).map (fun state => {x with state}) id
+
+/-- `pure a` gives a trivial coroutine, which completes in a single step, yielding the value `a` -/
+def pure (a : α) : CoroutineM α where
+  state := ()
+  next _ := .inr a
+
+/-- `map f x` applies a pure function `f : α → β` to the final result of state machine `x`,
+after it has completed. -/
+def map {α β : Type u} (f : α → β) (x : CoroutineM α) : CoroutineM β where
+  state  := x.state
+  next s := x.next s |>.map id f
+
+/-- `bind x f`, composes two state machines together, by running `f` after `x` completes,
+where the second state machine, `f`, may depend on the result of `x`  -/
+def bind {α β : Type u} (x : CoroutineM α) (f : α → CoroutineM β) : CoroutineM β where
+  σ := x.σ ⊕ Σ (a : α), (f a).σ × ((f a).σ → (f a).σ ⊕ β)
+  -- /-^^^---^^^^^^^^^^^^^^^^^^
+  -- | The state of `bind x f` is the sum of states of `x` and `f`
+  -- | However, `f` is a *function*, not a straight state machine,
+  -- | so read "the states of `f`" as:
+  -- |   "the infinite sum of all state types `(f x').σ`, for all possible values `a : α`"
+  state := .inl x.state
+  next := fun
+    | .inl (s : x.σ) =>
+      .inl <| (x.next s).map id (fun a => ⟨_, (f a).state, (f a).next⟩)
+        --  /----------------^^-----------^^^^^^^^^^^^^^^^^^^^^^^^^^^
+        --  | If `x` is still going, step into the next state of `x`,
+        --  |
+        --  | Otherwise, if `x` has completed, and yielded some value `a`,
+        --  | step into the first state of `f` that corresponds to `a`.
+        --  | Additionally, we store the transition function, so that we don't have to recompute it
+        --  | at every step
+    | .inr ⟨a, s, next⟩ => (next s).map (.inr ⟨a, ·, next⟩) id
+    -- ^^^^^^^^^^ Finally, run `f` until completion, mapping its state into
+    --            the combined sum state each step
+
+
+instance : Monad (CoroutineM) where
+  pure := pure
+  bind := bind
+
+
+end CoroutineM
