PartialMonad/CoroutineM/Bisim.lean
@@ -1,0 +1,85 @@
+import PartialMonad.CoroutineM
+
+/-!
+This file establishes a notion of bisimilarity on `CoroutineM`, and shows that is an equivalence
+relation
+-/
+
+namespace CoroutineM
+
+inductive StepAgrees (R : σ₁ → σ₂ → Prop) : σ₁ ⊕ α → σ₂ ⊕ α → Prop
+  | inl {s₁ s₂} : R s₁ s₂ → StepAgrees R (.inl s₁) (.inl s₂)
+  | inr {a} : StepAgrees R (.inr a) (.inr a)
+
+def IsBisimulation {x y : CoroutineM α} (R : x.σ → y.σ → Prop) : Prop :=
+  ∀ (s₁ : x.σ) (s₂ : y.σ), R s₁ s₂ → StepAgrees R (x.next s₁) (y.next s₂)
+
+inductive Bisim (x y : CoroutineM α) : Prop where
+  | mk
+    (R : x.σ → y.σ → Prop)
+    (bisim : IsBisimulation R)
+    (state : R x.state y.state)
+
+/-! `Bisim` is an equivalence -/
+section BisimIsEquiv
+
+theorem StepAgrees.rfl (h : ∀ a, R a a) : StepAgrees R x x := by
+  cases x <;> constructor
+  exact h _
+
+/-- `Eq` is a bisimulation -/
+theorem isBisimulation_eq {x : CoroutineM α} : @IsBisimulation _ x x Eq := by
+  simp only [IsBisimulation, forall_eq', implies_true, StepAgrees.rfl]
+
+namespace Bisim
+
+theorem rfl (x : CoroutineM α) : Bisim x x :=
+  .mk Eq isBisimulation_eq (by rfl)
+
+theorem trans : Bisim x y → Bisim y z → Bisim x z
+  | ⟨R₁, bisim₁, state₁⟩, ⟨R₂, bisim₂, state₂⟩ =>
+    .mk
+      (R := fun x z => ∃ y, R₁ x y ∧ R₂ y z)
+      (state := ⟨y.state, state₁, state₂⟩)
+      (bisim := by
+        intro s₁ s₃
+        simp
+        intro s₂ hR₁ hR₂
+        specialize bisim₁ _ _ hR₁; revert bisim₁
+        specialize bisim₂ _ _ hR₂; revert bisim₂
+
+        rcases x.next s₁ with s₁'|a₁
+        <;> rcases y.next s₂ with s₂'|a₂
+        <;> rcases z.next s₃ with s₃'|a₃
+        <;> rintro ⟨next₂⟩ ⟨next₁⟩
+        <;> constructor
+        exact ⟨_, next₁, next₂⟩
+      )
+
+theorem symm : Bisim x y → Bisim y x
+  | ⟨R, bisim, state⟩ =>
+      .mk (R := fun s₂ s₁ => R s₁ s₂) (state := state) (bisim := by
+        intros s₁ s₂ hR
+        specialize bisim _ _ hR
+        revert bisim
+        cases x.next s₂ <;> cases y.next s₁
+        <;> rintro ⟨bisim⟩
+        <;> constructor
+        assumption
+      )
+
+def equivalence : Equivalence (Bisim (α := α)) where
+  refl := rfl
+  trans := trans
+  symm := symm
+
+end Bisim
+
+/-- The canonical equality on coroutines is bisimilarity -/
+instance setoid (α : Type _) : Setoid (CoroutineM α) where
+  r := Bisim
+  iseqv := Bisim.equivalence
+
+end BisimIsEquiv
+
+end CoroutineM
