PartialMonad/CoroutineM/Get.lean
@@ -1,0 +1,70 @@
+import PartialMonad.CoroutineM
+
+/-!
+# Extracting Values From Coroutines
+
+* `CoroutineM.Terminates x` holds if the coroutine `x` terminates in finite time, and
+* `CoroutineM.getOfTerminates x h`, which runs `x` until completion, given a proof `h` that this will
+    happen in finite time
+-/
+
+namespace CoroutineM
+
+def iterate (x : CoroutineM α) : Nat → CoroutineM α ⊕ α
+  | 0   => .inl x
+  | n+1 => match x.nextState with
+      | .inl x' => x'.iterate n
+      | .inr a  => .inr a
+
+def Terminates (x : CoroutineM α) : Prop :=
+  ∃ n, (x.iterate n).isRight
+
+/-- `x.minimumStepsToTerminate h` is the smallest number `n`, such that `x` terminates in `n` steps -/
+protected noncomputable def minimumStepsToTerminate (x : CoroutineM α) (h : x.Terminates)  : Nat :=
+  go h.choose
+where go : Nat → Nat
+  | 0 => 0
+  | n+1 => match x.iterate n with
+    | .inl _ => n+1
+    --^^^^^^ `x` does *not* terminate in `n` steps, so `n+1` is the minimum
+    | .inr _ => go n
+    --^^^^^^ `x` still terminates in `n` steps, so try to minimize further
+
+/-- If `x'` is the next state of `x`, then we know that `x` takes exactly one more step to terminate
+than `x'` -/
+theorem minimumStepsToTerminate_le_of_eq {x x' : CoroutineM α}
+      (h_eq : x.nextState = .inl x') (h_terminates : x.Terminates) (h_terminates' : x'.Terminates) :
+    x.minimumStepsToTerminate h_terminates = x'.minimumStepsToTerminate h_terminates' + 1 := by
+  unfold CoroutineM.minimumStepsToTerminate
+  have n_spec := h_terminates.choose_spec
+  generalize h_terminates.choose = n at *
+  have n'_spec := h_terminates'.choose_spec
+  generalize h_terminates'.choose = n' at *
+
+  cases n
+  case zero => sorry
+  case succ n =>
+    simp [CoroutineM.minimumStepsToTerminate.go]
+    sorry
+
+def getOfTerminates (x : CoroutineM α) (h_terminates : x.Terminates) : α :=
+  match h_nextState : x.nextState with
+    | .inl x' =>
+        have h_terminates' := by
+          rcases h_terminates with ⟨n, h⟩
+          cases n
+          case zero =>
+            simp [iterate] at h
+          case succ n =>
+            simp [iterate, h_nextState] at h
+            exact ⟨_, h⟩
+        have :  x'.minimumStepsToTerminate h_terminates'
+                < x.minimumStepsToTerminate h_terminates := by
+          simp [minimumStepsToTerminate_le_of_eq h_nextState h_terminates h_terminates']
+        x'.getOfTerminates h_terminates'
+
+    | .inr a => a
+termination_by x.minimumStepsToTerminate h_terminates
+
+
+end CoroutineM
