PartialMonad/LawfulCoroutineM.lean
@@ -1,0 +1,45 @@
+import PartialMonad.CoroutineM
+import PartialMonad.CoroutineM.Bisim
+import PartialMonad.CoroutineM.Get
+
+/-!
+This file defines the `LawfulCoroutineM` monad.
+
+As the name suggests, this is a lawful version of `CoroutineM`, it is constructed by quotienting
+coroutines through the bisimilarity relation.
+-/
+
+#check ULift
+
+def CoroutineM.bumpUniverse.{r, s} {α : Type s} (x : CoroutineM.{s} α) :
+    CoroutineM.{r} (ULift.{r, s} α) where
+  σ := ULift x.σ
+  state := .up x.state
+  next s := sorry
+
+def LawfulCoroutineM (α : Type u) := Quotient (CoroutineM.setoid α)
+
+namespace LawfulCoroutineM
+
+/-- The canonical map from `CoroutineM` into the quotient -/
+def ofCoroutine : CoroutineM α → LawfulCoroutineM α :=
+  Quotient.mk _
+
+/-- `pure a` gives a trivial coroutine, which completes in a single step, yielding the value `a` -/
+def pure (a : α) : LawfulCoroutineM α :=
+  ofCoroutine <| CoroutineM.pure a
+
+
+/-
+Now comes the tricky part, how are we going to define `bind`
+-/
+
+def bind {α β : Type u} (x : LawfulCoroutineM α) (f : α → LawfulCoroutineM β) :
+    LawfulCoroutineM β :=
+  let f_lift (x : CoroutineM α) : LawfulCoroutineM β :=
+    let x' := x.map f
+    sorry
+  Quotient.liftOn x f_lift _
+
+
+end LawfulCoroutineM
