lakefile.lean
@@ -7,6 +7,8 @@ package «partial-monad» where
 lean_lib «PartialMonad» where
   -- add library configuration options here
 
+require std from git "https://github.com/leanprover/std4" @ "main"
+
 @[default_target]
 lean_exe «partial-monad» where
   root := `Main
